checkpoint experiments

TotalSemantics.thy
@@ -3,7 +3,6 @@ imports Viper.ViperLang TotalExpressions
 begin
 
 datatype fail = WellDefFail | StandardFail
-datatype 'a inh_exh_result = IEFailure fail | Set "'a full_total_state set"
 
 datatype 'a result = Failure | Set (select_set: "'a full_total_state set")
 
@@ -22,9 +21,14 @@ fun update_store_total :: "'a full_total_state \<Rightarrow> var \<Rightarrow> '
 definition update_heap_total :: "'a total_state \<Rightarrow> heap_loc \<Rightarrow> 'a val \<Rightarrow> 'a total_state"
   where "update_heap_total mh l v = Abs_total_state ((get_mask_total mh), (get_heap_total mh)(l := v))"
 
+definition update_mask_total :: "'a total_state \<Rightarrow> mask \<Rightarrow> 'a total_state"
+  where "update_mask_total mh m' = Abs_total_state (m', get_heap_total mh)"
+
 fun update_heap_total_full :: "'a full_total_state \<Rightarrow> heap_loc \<Rightarrow> 'a val \<Rightarrow> 'a full_total_state"
   where "update_heap_total_full (\<sigma>, \<pi>, \<phi>) l v = (\<sigma>, \<pi>, update_heap_total \<phi> l v )"
 
+fun update_mask_total_full :: "'a full_total_state \<Rightarrow> mask \<Rightarrow> 'a full_total_state"
+  where "update_mask_total_full (\<sigma>, \<pi>, \<phi>) m = (\<sigma>, \<pi>, update_mask_total \<phi> m)" 
 
 definition singleton_total_pred :: "heap_loc \<Rightarrow> (prat \<Rightarrow> 'a val \<Rightarrow> bool) \<Rightarrow> 'a store \<Rightarrow> 'a total_trace \<Rightarrow> ('a full_total_state) set"
   where "singleton_total_pred l P \<sigma> \<tau> = { (\<sigma>, \<tau>, Abs_total_state (m,h)) |m h. P (m l) (h l)}"
@@ -40,13 +44,35 @@ fun map_result :: "(('a full_total_state) \<Rightarrow> 'a result) \<Rightarrow>
     "map_result f Failure = Failure"
   | "map_result f (Set xs) = (if \<exists>x \<in> xs. f x = Failure then Failure else Set (\<Union>x \<in> xs. select_set (f x))) "
 
+fun map_result_2 :: "(mask \<Rightarrow> (mask set) option) \<Rightarrow> (mask set) option \<Rightarrow> (mask set) option"
+  where 
+    "map_result_2 f None = None"
+  | "map_result_2 f (Some xs) = (if \<exists>x \<in> xs. f x = None then None else Some (\<Union>x \<in> xs. the (f x))) "
+
+
 fun get_address_opt :: "'a val \<Rightarrow> address option"
   where 
     "get_address_opt (VRef (Address a)) = Some a"
   | "get_address_opt _ = None"
 
 
-fun handle_inhale :: "'a program \<Rightarrow> bool \<Rightarrow> bool \<Rightarrow> assertion \<Rightarrow> 'a full_total_state \<Rightarrow> 'a result"
+datatype 'a inh_exh_result = InhExhFailure | InhExhNormal "'a full_total_state"
+
+(*
+inductive red_inhale :: "program \<Rightarrow> bool \<Rightarrow> bool \<Rightarrow> assertion \<Rightarrow> 'a full_total_state \<Rightarrow>  'a inh_exh_result \<Rightarrow> bool"
+  where 
+   "\<lbrakk> red_inhale Pr havoc_new inh_assume A \<omega> (InhExhNormal \<omega>''); 
+      red_inhale Pr havoc_new inh_assume B \<omega>'' (InhExhNormal \<omega>')\<rbrakk> \<Longrightarrow>
+    red_inhale Pr havoc_new inh_assume (A && B) \<omega> (InhExhNormal \<omega>')"
+ | "\<lbrakk> red_inhale Pr havoc_new inh_assume A \<omega> InhExhFailure \<rbrakk> \<Longrightarrow>
+    red_inhale Pr havoc_new inh_assume (A && B) \<omega> InhExhFailure"
+ | "\<lbrakk> red_inhale Pr havoc_new inh_assume A \<omega> (InhExhNormal \<omega>''); 
+      red_inhale Pr havoc_new inh_assume B \<omega>'' InhExhFailure \<rbrakk> \<Longrightarrow>
+    red_inhale Pr havoc_new inh_assume (A && B) \<omega> InhExhFailure"
+ | "\<lbrakk> a_opt = get_address_opt (red_pure_exp_total Pr e_r \<omega>); p = (un_VPerm (red_pure_exp_total Pr e_p \<omega>)) \<rbrakk> \<Longrightarrow>
+*)
+
+fun handle_inhale :: "program \<Rightarrow> bool \<Rightarrow> bool \<Rightarrow> assertion \<Rightarrow> 'a full_total_state \<Rightarrow> 'a result"
   where 
 (** Connectives **)
     "handle_inhale Pr havoc_new inh_assume (A && B) \<omega> = 
@@ -99,7 +125,7 @@ fun handle_inhale :: "'a program \<Rightarrow> bool \<Rightarrow> bool \<Rightar
   | "handle_inhale Pr havoc_new inh_assume (A --* B) \<omega> = undefined"
 
 
-fun handle_exhale :: "'a program \<Rightarrow> heap_loc set \<Rightarrow> assertion \<Rightarrow> 'a full_total_state \<Rightarrow> 'a result"
+fun handle_exhale :: "program \<Rightarrow> heap_loc set \<Rightarrow> assertion \<Rightarrow> 'a full_total_state \<Rightarrow> 'a result"
   where
     "handle_exhale Pr def_locs (A && B) \<omega> = 
        map_result (handle_exhale Pr def_locs B) (handle_exhale Pr def_locs A \<omega>)"
@@ -131,157 +157,317 @@ fun handle_exhale :: "'a program \<Rightarrow> heap_loc set \<Rightarrow> assert
   | "handle_exhale Pr def_locs (Atomic (AccPredicateWildcard va vb)) \<omega> = undefined"
   | "handle_exhale Pr def_locs (A --* B) \<omega> = undefined"
 
-record conf =
-  havoc_inhale :: bool
-
-type_synonym 'a stmt_config = "(stmt+unit) \<times> ('a result)"
 
 definition get_valid_locs :: "'a full_total_state \<Rightarrow> heap_loc set"
   where "get_valid_locs \<omega> = {l |l. pgt (get_mask_total_full \<omega> l) pnone}"
 
-inductive red_stmt_total_single :: "'a program \<Rightarrow> conf \<Rightarrow> stmt \<Rightarrow> 'a full_total_state  \<Rightarrow> 'a stmt_config \<Rightarrow> bool" where
-   RedSkip: " red_stmt_total_single Pr conf Skip \<omega> (Inr (), Set {\<omega>})"
- | RedInhale: "red_stmt_total_single Pr conf (Inhale A) \<omega> (Inr (), (handle_inhale Pr (havoc_inhale conf) False A \<omega>))"
- | RedAssume: "red_stmt_total_single Pr conf (Assume A) \<omega> (Inr (), (handle_inhale Pr (havoc_inhale conf) True A \<omega>))"
- | RedExhale: "red_stmt_total_single Pr conf (Exhale A) \<omega> (Inr (), (handle_exhale Pr (get_valid_locs \<omega>) A \<omega>))"
- | RedSeq1: "\<lbrakk> red_stmt_total_single Pr conf s1 \<omega> (Inl s'', r'') \<rbrakk> \<Longrightarrow>
-               red_stmt_total_single Pr conf (Seq s1 s2) \<omega> (Inl (Seq s'' s2), r'')"
- | RedSeq2: "\<lbrakk> red_stmt_total_single Pr conf s1 \<omega> (Inr (), r'') \<rbrakk> \<Longrightarrow>
-               red_stmt_total_single Pr conf (Seq s1 s2) \<omega> (Inl s2, r'')"
+fun handle_exhale_2 :: "program \<Rightarrow> 'a full_total_state \<Rightarrow> assertion \<Rightarrow> mask \<Rightarrow> (mask set) option"
+  where
+    "handle_exhale_2 Pr \<omega>_orig (A && B) m = 
+       map_result_2 (handle_exhale_2 Pr \<omega>_orig B) (handle_exhale_2 Pr \<omega>_orig A m)"
+  | "handle_exhale_2 Pr \<omega>_orig (Imp e A) m = 
+       (if (red_pure_exp_total Pr e (update_mask_total_full \<omega>_orig m)) = VBool True then (handle_exhale_2 Pr \<omega>_orig A m) else Some {m})"
+  | "handle_exhale_2 Pr \<omega>_orig (Atomic (Acc e_r f e_p)) m = 
+       (let \<omega> = (update_mask_total_full \<omega>_orig m);
+            a_opt = get_address_opt (red_pure_exp_total Pr e_r \<omega>);
+            p = (un_VPerm (red_pure_exp_total Pr e_p \<omega>)) 
+        in            
+            if (p \<ge> 0 \<and> (wd_pure_exp_total Pr (CExhale (get_valid_locs \<omega>_orig)) e_r \<omega>) \<and> a_opt \<noteq> None) \<and> pgte (get_mask_total_full \<omega> ((the a_opt),f) ) (Abs_prat p) then            
+             Some  { ( m(((the a_opt),f) := Abs_prat ( (Rep_prat (m((the a_opt, f)))) - p)) ) }
+            else 
+             None)     
+      "
+  | "handle_exhale_2 Pr \<omega>_orig (Atomic (AccWildcard e_r f)) m =
+       (let \<omega> = (update_mask_total_full \<omega>_orig m);
+            a_opt = get_address_opt (red_pure_exp_total Pr e_r \<omega>);
+            cur_p = m(the a_opt, f)
+        in 
+          if ((wd_pure_exp_total Pr (CExhale (get_valid_locs \<omega>)) e_r \<omega>) \<and> a_opt \<noteq> None) \<and> pgt cur_p pnone then
+             Some {m((the a_opt,f) := Abs_prat((Rep_prat cur_p) - p'))| p'. p' > 0 \<and> p' < Rep_prat cur_p}
+          else None)"
+  | "handle_exhale_2 Pr \<omega>_orig (InhaleExhale A B) m = handle_exhale_2 Pr \<omega>_orig B m"
+  | "handle_exhale_2 Pr \<omega>_orig (Atomic (Pure e)) m =
+         (let \<omega> = (update_mask_total_full \<omega>_orig m) in
+          (if wd_pure_exp_total Pr (CExhale (get_valid_locs \<omega>)) e \<omega> \<and> (un_VBool (red_pure_exp_total Pr e \<omega>)) then 
+              Some {m}
+          else None))"
+  | "handle_exhale_2 Pr \<omega>_orig (ForAll v va) \<omega> = undefined"
+  | "handle_exhale_2 Pr \<omega>_orig (Atomic (AccPredicate va vb vc)) \<omega> = undefined"
+  | "handle_exhale_2 Pr \<omega>_orig (Atomic (AccPredicateWildcard va vb)) \<omega> = undefined"
+  | "handle_exhale_2 Pr \<omega>_orig (A --* B) \<omega> = undefined"
+
+record conf =
+  havoc_inhale :: bool
+
+
+(* alt:
+definition havoc_undef_locs :: "'a full_total_state \<Rightarrow> mask \<Rightarrow> 'a full_total_state set"
+  where "havoc_undef_locs \<omega> m = {\<omega>'| \<omega>'. \<forall>l. pgt (m l) pnone \<longrightarrow> get_heap_total_full \<omega> l = get_heap_total_full \<omega>' l}"
+*)
+definition havoc_undef_locs :: "'a total_heap \<Rightarrow> mask \<Rightarrow> 'a total_heap set"
+  where "havoc_undef_locs h m = {h' | h'. \<forall>l. pgt (m l) pnone \<longrightarrow> h' l = h l}"
+
+definition exhale_state :: "'a full_total_state \<Rightarrow> mask \<Rightarrow> 'a full_total_state set"
+  where "exhale_state \<omega> m = {\<omega>' | \<omega>'. get_store_total \<omega>' = get_store_total \<omega> \<and>
+                                      get_trace_total \<omega>' = get_trace_total \<omega> \<and>
+                                      get_mask_total_full \<omega>' = m \<and>
+                                      get_heap_total_full \<omega>' \<in> havoc_undef_locs (get_heap_total_full \<omega>) m}"
+
+
+fun map_option_2 :: "('a \<Rightarrow> 'b) \<Rightarrow> 'b \<Rightarrow> 'a option \<Rightarrow> 'b"
+  where 
+    "map_option_2 f y None = y"
+  | "map_option_2 f _ (Some x) = f x"
+      
+
+(* Currently, red_stmt_total_single is a function. But if angelism is added, then it would not be a 
+function *)
+inductive red_stmt_total_single_set :: "program \<Rightarrow> conf \<Rightarrow> stmt \<Rightarrow> 'a full_total_state  \<Rightarrow> (stmt+unit) \<times> ('a result) \<Rightarrow> bool" where
+   RedSkip: " red_stmt_total_single_set Pr conf Skip \<omega> (Inr (), Set {\<omega>})"
+ | RedInhale: "red_stmt_total_single_set Pr conf (Inhale A) \<omega> (Inr (), (handle_inhale Pr (havoc_inhale conf) False A \<omega>))"
+ | RedAssume: "red_stmt_total_single_set Pr conf (Assume A) \<omega> (Inr (), (handle_inhale Pr (havoc_inhale conf) True A \<omega>))"
+ | RedExhale: "red_stmt_total_single_set Pr conf (Exhale A) \<omega> 
+                     (Inr (), map_option_2 (\<lambda>xs. Set (\<Union>m \<in> xs. exhale_state \<omega> m)) Failure (handle_exhale_2 Pr \<omega> A (get_total_mask_full \<omega>)))"
+ | RedSeq1: "\<lbrakk> red_stmt_total_single_set Pr conf s1 \<omega> (Inl s'', r'') \<rbrakk> \<Longrightarrow>
+               red_stmt_total_single_set Pr conf (Seq s1 s2) \<omega> (Inl (Seq s'' s2), r'')"
+ | RedSeq2: "\<lbrakk> red_stmt_total_single_set Pr conf s1 \<omega> (Inr (), r'') \<rbrakk> \<Longrightarrow>
+               red_stmt_total_single_set Pr conf (Seq s1 s2) \<omega> (Inl s2, r'')"
  | RedLocalAssign: "\<lbrakk> wd_pure_exp_total Pr CInhale e \<omega>; Pr \<turnstile> \<langle>e; \<omega>\<rangle> [\<Down>]\<^sub>t = v \<rbrakk> \<Longrightarrow> 
-               red_stmt_total_single Pr conf (LocalAssign x e) \<omega> (Inr (), (Set {update_store_total \<omega> x v}))"
- | RedLocalAssignFailure: "\<lbrakk> \<not> wd_pure_exp_total Pr CInhale e \<omega> \<rbrakk> \<Longrightarrow> red_stmt_total_single Pr conf (LocalAssign x e) \<omega> (Inr (), Failure)"
+               red_stmt_total_single_set Pr conf (LocalAssign x e) \<omega> (Inr (), (Set {update_store_total \<omega> x v}))"
+ | RedLocalAssignFailure: "\<lbrakk> \<not> wd_pure_exp_total Pr CInhale e \<omega> \<rbrakk> \<Longrightarrow> red_stmt_total_single_set Pr conf (LocalAssign x e) \<omega> (Inr (), Failure)"
  | RedFieldAssign: "\<lbrakk> wd_pure_exp_total Pr CInhale e_r \<omega>; 
                       wd_pure_exp_total Pr CInhale e \<omega>; 
                       Pr \<turnstile> \<langle>e_r; \<omega>\<rangle> [\<Down>]\<^sub>t = VRef (Address addr);
                       Pr \<turnstile> \<langle>e; \<omega>\<rangle> [\<Down>]\<^sub>t = v \<rbrakk> \<Longrightarrow> 
-               red_stmt_total_single Pr conf (FieldAssign e_r f e) \<omega> (Inr (), (Set {update_heap_total_full \<omega> (addr,f) v}))"
+               red_stmt_total_single_set Pr conf (FieldAssign e_r f e) \<omega> (Inr (), (Set {update_heap_total_full \<omega> (addr,f) v}))"
  | RedFieldAssignFailure: "\<lbrakk> \<not> wd_pure_exp_total Pr CInhale e_r \<omega> \<or> \<not> wd_pure_exp_total Pr CInhale e \<omega> \<or> (Pr \<turnstile> \<langle>e_r; \<omega>\<rangle> [\<Down>]\<^sub>t) = (VRef Null) \<rbrakk> \<Longrightarrow> 
-               red_stmt_total_single Pr conf (FieldAssign e_r f e) \<omega> (Inr (), Failure)"
+               red_stmt_total_single_set Pr conf (FieldAssign e_r f e) \<omega> (Inr (), Failure)"
  | RedIfTrue: "\<lbrakk> Pr \<turnstile> \<langle>e_b; \<omega>\<rangle> [\<Down>]\<^sub>t = VBool True \<rbrakk> \<Longrightarrow> 
-                red_stmt_total_single Pr conf (If e_b s1 s2) \<omega> (Inl s1, Set {\<omega>})"
+                red_stmt_total_single_set Pr conf (If e_b s1 s2) \<omega> (Inl s1, Set {\<omega>})"
  | RedIfFalse: "\<lbrakk> Pr \<turnstile> \<langle>e_b; \<omega>\<rangle> [\<Down>]\<^sub>t = VBool False \<rbrakk> \<Longrightarrow> 
-                red_stmt_total_single Pr conf (If e_b s1 s2) \<omega> (Inl s2, Set {\<omega>})"
+                red_stmt_total_single_set Pr conf (If e_b s1 s2) \<omega> (Inl s2, Set {\<omega>})"
 
+(* datatype 'a stmt_config_2 = Failure2 | Normal "((stmt + unit) \<times> 'a full_total_state) set" *)
 
-(*
+type_synonym 'a stmt_config = "(stmt + unit) \<times> 'a full_total_state"
 
-type_synonym config2 = " (stmt + unit, state set)  + 'a result
-fun red_stmt_total_single_2 :: "'a program \<Rightarrow> conf \<Rightarrow> ('a stmt_config) set \<Rightarrow> ('a stmt_config) set"
-  where "red_stmt_total_single_2 Pr c W W' = 
-*)
+datatype 'a single_result = FailureSingle | Normal "(stmt + unit) \<times> 'a full_total_state"
 
-datatype 'a stmt_config_2 = Failure | Set "( (stmt + unit) \<times> 'a full_total_state) set"
-
-(*
-fun small_step_2 :: "'a program \<Rightarrow> conf \<Rightarrow> 'a stmt_config_2 \<Rightarrow> 'a stmt_config_2"
+inductive red_stmt_total_single :: "program \<Rightarrow> conf \<Rightarrow> 'a single_result \<Rightarrow> 'a single_result \<Rightarrow> bool"
   where 
-    "small_step_2 Pr c Failure = Failure"
-  | "small_step_2 Pr c (Set W) =
-*)
+    NormalSingleStep: "\<lbrakk> red_stmt_total_single_set Pr conf s \<omega> (m', Set W'); \<omega>' \<in> W' \<rbrakk> \<Longrightarrow> 
+       red_stmt_total_single Pr conf (Normal (Inl s, \<omega>)) (Normal (m', \<omega>'))"
+  | FailureSingleStep: "\<lbrakk> red_stmt_total_single_set Pr conf s \<omega> (m', Failure) \<rbrakk> \<Longrightarrow>
+       red_stmt_total_single Pr conf (Normal (Inl s, \<omega>)) FailureSingle"
 
-(*
-inductive red_stmt_total_single_2 :: "'a program => conf \<Rightarrow> 'a stmt_config \<Rightarrow> 'a stmt_config \<Rightarrow> bool"
+definition red_stmt_total_multi :: "program \<Rightarrow> conf \<Rightarrow> 'a single_result \<Rightarrow> 'a single_result \<Rightarrow> bool"
+  where "red_stmt_total_multi Pr conf = rtranclp (red_stmt_total_single Pr conf)"
+
+
+definition is_empty_total :: "'a full_total_state \<Rightarrow> bool"
+  where "is_empty_total \<omega> \<equiv> get_mask_total_full \<omega> = zero_mask"
+
+(* todo: incorporate precondition *)
+(* first argument is just there to fix 'a *)
+definition stmt_verifies_total :: "'a full_total_state \<Rightarrow> program \<Rightarrow> conf \<Rightarrow> stmt \<Rightarrow>  bool"
+  where "stmt_verifies_total dummy Pr conf s \<equiv> 
+         \<forall>(\<omega> :: 'a full_total_state) r. is_empty_total \<omega> \<longrightarrow> 
+           red_stmt_total_multi Pr conf ((Normal (Inl s, \<omega>))) r \<longrightarrow> r \<noteq> FailureSingle"
+
+
+subsection \<open>Havoc at exhale is sufficient\<close>
+
+definition equal_on_mask :: "mask \<Rightarrow> 'a total_heap \<Rightarrow> 'a total_heap \<Rightarrow> bool"
+  where "equal_on_mask m h1 h2 \<equiv> \<forall> l. m(l) \<noteq> pnone \<longrightarrow> h1(l) = h2(l)"
+
+lemma equal_on_mask_refl: "equal_on_mask m h h"
+  by (simp add: equal_on_mask_def)
+
+type_synonym 'a simulation_rel = "'a full_total_state \<Rightarrow> 'a full_total_state \<Rightarrow> bool"
+
+lemma havoc_equiv:
+  assumes "stmt_verifies_total dummy Pr \<lparr>havoc_inhale = false\<rparr> s"
+  shows "stmt_verifies_total dummy Pr \<lparr>havoc_inhale = true\<rparr> s"
+  oops
+
+  subsection \<open>Backwards simulation\<close>
+
+(*definition lift_simulation_rel :: "'a simulation_rel \<Longrightarrow> *)
+
+lemma backwards_simulation:
+  assumes initial_rel: "\<And> \<omega> \<omega>2. is_empty_total \<omega> \<Longrightarrow> R \<omega> \<omega>2 \<Longrightarrow> is_empty_total \<omega>2" and
+          total_rel: "\<forall>\<omega>. \<exists> \<omega>'. R \<omega> \<omega>'" and
+          step:"\<And> s \<omega> w. red_stmt_total_single Pr conf (Normal (Inl s, \<omega>)) w \<Longrightarrow>
+                (w = FailureSingle \<longrightarrow> (\<exists>\<omega>2. R \<omega> \<omega>2 \<and> red_stmt_total_single Pr2 conf2 (Normal (Inl s, \<omega>2)) FailureSingle)) \<and>
+                (\<forall> s' \<omega>' \<omega>2'. (w = Normal (Inl s', \<omega>') \<longrightarrow> R \<omega>' \<omega>2' \<longrightarrow>
+                               (\<exists>\<omega>2. R \<omega> \<omega>2 \<and> red_stmt_total_single Pr2 conf2 (Normal (Inl s, \<omega>2)) (Normal (Inl s', \<omega>2')))))"
+        assumes "stmt_verifies_total dummy Pr2 conf2 s"
+ shows "stmt_verifies_total dummy Pr conf s"
+  sorry
+
+definition havoc_rel :: "'a simulation_rel"
+  where "havoc_rel \<omega> \<omega>' \<equiv> get_mask_total_full \<omega> = get_mask_total_full \<omega>' \<and> 
+                          equal_on_mask (get_mask_total_full \<omega>) (get_heap_total_full \<omega>) (get_heap_total_full \<omega>')"
+
+lemma init_havoc_rel: "is_empty_total \<omega> \<Longrightarrow> havoc_rel \<omega> \<omega>2 \<Longrightarrow> is_empty_total \<omega>2"
+  by (simp add: havoc_rel_def is_empty_total_def)
+
+lemma total_havoc_rel: "\<exists> \<omega>'. havoc_rel \<omega> \<omega>'"
+  by (rule exI[where ?x=\<omega>]) (simp add: havoc_rel_def equal_on_mask_refl)
+
+fun supported_subset :: "assertion \<Rightarrow> bool"
   where 
-    RedFailureProp: "red_stmt_total_single_2 Pr c (m, Failure) (Inr (), Failure)"
-  | RedFailure: "\<lbrakk> \<omega> \<in> W; red_stmt_total_single Pr c s1 \<omega> (m, Failure) \<rbrakk> \<Longrightarrow>
-                 red_stmt_total_single_2 Pr c (Inl s1, Set W) (Inr (), Failure)"
-  | RedNormal: " \<lbrakk> W' = (\<Union>\<omega>\<in>W. {W' | W'. red_stmt_total_single Pr c s1 \<omega>  (Set W')}) \<rbrakk> \<Longrightarrow>
-                red_stmt_total_single_2 Pr c (Inl s1, Set W) (Inr (), Set W')"
+    "supported_subset (ForAll v va) = False"
+  | "supported_subset (Atomic (AccPredicate va vb vc)) = False"
+  | "supported_subset (Atomic (AccPredicateWildcard va vb)) = False"
+  | "supported_subset (A --* B) = False"
+  | "supported_subset _ = True"
+
+
+lemma test: 
+  assumes "handle_inhale Pr h inh_assume (A&&B) \<omega> = Set W'" and "\<omega>' \<in> W'"
+  shows "\<exists>W'' \<omega>'' W2'. handle_inhale Pr h inh_assume A \<omega> = Set W'' \<and> \<omega>'' \<in> W'' \<and> handle_inhale Pr h inh_assume B \<omega>'' = Set W2' \<and> \<omega>' \<in> W2'"
+  oops
+
+lemma havoc_inhale_rel:
+  assumes "handle_inhale Pr True inh_assume A \<omega> = Set W'" and "\<omega>' \<in> W'" and "havoc_rel \<omega>' \<omega>2'" (*and "supported_subset A"*)
+  shows "handle_inhale Pr False inh_assume A (update_mask_total_full \<omega>2' (get_mask_total_full \<omega>)) = Set {\<omega>2'}"
+  using assms
+proof (induction Pr True inh_assume A \<omega> arbitrary:W' \<omega>' \<omega>2' rule: handle_inhale.induct)
+  case (1 Pr inh_assume A B \<omega>)
+  from \<open>handle_inhale Pr True inh_assume (A && B) \<omega> = Set W'\<close> 
+then show ?case sorry
+next
+  case (2 Pr inh_assume e A \<omega>)
+  then show ?case sorry
+next
+  case (3 Pr e_r f e_p \<omega>)
+  then show ?case sorry
+next
+  case (4 Pr e_r f \<omega>)
+  then show ?case sorry
+next
+  case (5 Pr e_r f e_p \<omega>)
+  then show ?case sorry
+next
+  case (6 Pr e_r f \<omega>)
+  then show ?case sorry
+next
+  case (7 Pr inh_assume A B \<omega>)
+  then show ?case sorry
+next
+  case (8 Pr inh_assume e \<omega>)
+  then show ?case sorry
+next
+  case (9 Pr inh_assume v va \<omega>)
+  then show ?case sorry
+next
+  case (10 Pr inh_assume va vb vc \<omega>)
+  then show ?case sorry
+next
+  case (11 Pr inh_assume va vb \<omega>)
+  then show ?case sorry
+next
+  case (12 Pr inh_assume A B \<omega>)
+  then show ?case sorry
+qed
+
+
+
+lemma step_havoc_rel:
+  assumes "red_stmt_total_single Pr \<lparr>havoc_inhale=False\<rparr> (Normal (Inl s, \<omega>)) w"
+  shows   "(w = FailureSingle \<longrightarrow> (\<exists>\<omega>2. R \<omega> \<omega>2 \<and> red_stmt_total_single Pr \<lparr>havoc_inhale=False\<rparr> (Normal (Inl s, \<omega>2)) FailureSingle)) \<and>
+                (\<forall> s' \<omega>' \<omega>2'. (w = Normal (Inl s', \<omega>') \<longrightarrow> R \<omega>' \<omega>2' \<longrightarrow>
+                               (\<exists>\<omega>2. R \<omega> \<omega>2 \<and> red_stmt_total_single Pr \<lparr>havoc_inhale=False\<rparr> (Normal (Inl s, \<omega>2)) (Normal (Inl s', \<omega>2')))))"
+  using assms
+proof (cases)
+  case (NormalSingleStep m' W' \<omega>')
+  from NormalSingleStep(2) show ?thesis 
+  proof cases
+  case RedSkip
+  show ?thesis
+    by (simp add: local.NormalSingleStep(1) local.RedSkip(2))
+  next
+    case (RedInhale A)
+    then show ?thesis sorry
+  next
+  case (RedAssume A)
+    then show ?thesis sorry
+  next
+    case (RedExhale A get_total_mask_full)
+    then show ?thesis sorry
+  next
+  case (RedSeq1 s1 s'' s2)
+  then show ?thesis sorry
+  next
+  case (RedSeq2 s1 s2)
+  then show ?thesis sorry
+  next
+    case (RedLocalAssign e v x)
+    then show ?thesis sorry
+  next
+  case (RedFieldAssign e_r e addr v f)
+    then show ?thesis sorry
+  next
+    case (RedIfTrue e_b s1 s2)
+    then show ?thesis sorry
+  next
+    case (RedIfFalse e_b s1 s2)
+    then show ?thesis sorry
+  qed
+next
+  case (FailureSingleStep m')
+  then show ?thesis sorry
+qed
+
+lemma havoc_conf_equiv:
+  assumes "stmt_verifies_total dummy Pr \<lparr>havoc_inhale=False\<rparr> s"
+  shows "stmt_verifies_total dummy Pr \<lparr>havoc_inhale=True\<rparr> s"
+proof (rule backwards_simulation)
+  
+  
+
+
+
+
+(*
+inductive red_stmt_total_single_2 :: "'a program \<Rightarrow> conf \<Rightarrow> stmt \<Rightarrow> 'a stmt_config_2  \<Rightarrow> 'a stmt_config_2 \<Rightarrow> bool" where
+  "red_stmt_total_single_2 Pr conf s Normal C1 C2 =
+         (\<forall> "
+*)
+
+(*datatype 'a stmt_config_2 = SmallStepFailure | Normal "( (stmt + unit) \<times> 'a result) set"*)
+
+(*type_synonym 'a stmt_config_3 = "((stmt + unit) \<times> *)
+(*
+fun small_step_lifted :: "'a program \<Rightarrow> conf \<Rightarrow> 'a stmt_config_2 \<Rightarrow> 'a stmt_config_2 \<Rightarrow> bool"
+  where 
+    "small_step_lifted Pr conf S S' = 
+*)         
+(*
+  | "small_step_lifted Pr conf (Normal S) = 
+       (if (\<exists>s \<omega> m'. (Inl s, \<omega>) \<in> S \<and> red_stmt_total_single Pr conf s \<omega> (m', Failure)) then
+          SmallStepFailure
+       else 
+         Normal {(m', \<omega>') | s \<omega> m' \<omega>' W'. (Inl s, \<omega>) \<in> S \<and> \<omega>' \<in> W' \<and> red_stmt_total_single Pr conf s \<omega> (m', Set W')})"
+*)
+
+(*
+fun small_step_lifted :: "'a program \<Rightarrow> conf \<Rightarrow> 'a stmt_config_2 \<Rightarrow> 'a stmt_config_2"
+  where 
+    "small_step_lifted Pr conf SmallStepFailure = SmallStepFailure"
+  | "small_step_lifted Pr conf (Normal S) = 
+       (if (\<exists>s \<omega> m'. (Inl s, \<omega>) \<in> S \<and> red_stmt_total_single Pr conf s \<omega> (m', Failure)) then
+          SmallStepFailure
+       else 
+         Normal {(m', \<omega>') | s \<omega> m' \<omega>' W'. (Inl s, \<omega>) \<in> S \<and> \<omega>' \<in> W' \<and> red_stmt_total_single Pr conf s \<omega> (m', Set W')})"
 *)
 (*
-inductive red_stmt_total_2 :: "'a program \<Rightarrow> conf \<Rightarrow> 'a stmt_config \<Rightarrow> 'a stmt_config \<Rightarrow> bool" where 
-   RedSkip: " red_stmt_total_2 Pr conf ((Inl Skip), r) (Inr (), r)"
- | RedInhale: "red_stmt_total_2 Pr conf (Inl (Inhale A), (Set W)) (Inr (), \<Union>\<omega> \<in> W. (handle_inhale Pr (havoc_inhale conf) A \<omega>))"
- | RedSeq1: "\<lbrakk> red_stmt_total_2 Pr conf (Inl s1, (Set W)) (Inl s'', r'') \<rbrakk> \<Longrightarrow>
-               red_stmt_total_2 Pr conf (Inl (Seq s1 s2), (Set W)) (Inl (Seq s'' s2), r'')"
- | RedSeq2: "\<lbrakk> red_stmt_total_2 Pr conf (Inl s1, (Set W)) (Inr (), r'') \<rbrakk> \<Longrightarrow>
-               red_stmt_total_2 Pr conf (Inl (Seq s1 s2), (Set W)) (Inl s2, r'')"
- | RedFailure: "red_stmt_total_2 Pr conf ( (Inl s), Failure ) (Inr (), Failure)"
-*)
+definition small_step_multi :: "'a program \<Rightarrow> conf \<Rightarrow> 'a stmt_config_2 \<Rightarrow> 'a stmt_config_2 \<Rightarrow> bool"
+  where "small_step_multi Pr conf = rtranclp (small_step_lifted Pr conf)"
 
-  (* RedSeq: "red_stmt_total_2 Pr conf (Seq s1 s2) W (Set W')"*)
-
-
-inductive red_stmt_total :: "'a program \<Rightarrow> conf \<Rightarrow> stmt \<Rightarrow> 'a full_total_state \<Rightarrow> 'a result \<Rightarrow> bool" where
-  RedSkip: "red_stmt_total Pr conf Skip \<omega> (Set {\<omega>})"
-(*
-| RedAssertTrue: "\<lbrakk> wft Pr RExhale A \<omega> \<rbrakk> \<Longrightarrow> red_stmt conf Pr (Assert A) \<omega> (Set {\<omega>})"
-| RedAssertFalse: "\<lbrakk> wd_assertion Pr RExhale A \<omega> ; \<not> Pr RExhale \<Turnstile> \<langle>A; \<omega>\<rangle> \<rbrakk> \<Longrightarrow> red_stmt conf Pr (Assert A) \<omega> Failure"
-*)
-| RedInhale: "red_stmt_total Pr conf (Inhale A) \<omega> (handle_inhale Pr (havoc_inhale conf) A \<omega>)"
-| RedExhale: "red_stmt_total Pr conf (Exhale A) \<omega> (handle_exhale Pr {} A \<omega>)"
-| RedSeq: "\<lbrakk> red_stmt_total Pr conf s1 \<omega> (Set s) \<rbrakk> \<Longrightarrow> 
-             red_stmt_total Pr conf (Seq s1 s2) \<omega> (Set r)"
-
-
-(*
-| RedExhaleTrueAngelic: "\<lbrakk> angelic_exhale conf ; wft Pr RExhale A \<omega> ; a \<in> SA.under (inh Pr RExhale A) \<omega> \<rbrakk> \<Longrightarrow> red_stmt conf Pr (Exhale A) \<omega> (Set {\<omega> \<ominus> a})"
-| RedExhaleTrueDemonic: "\<lbrakk> \<not> angelic_exhale conf ; wft Pr RExhale A \<omega> \<rbrakk> \<Longrightarrow> red_stmt conf Pr (Exhale A) \<omega> (Set {(\<omega> \<ominus> a) |a. a \<in> SA.under (inh Pr RExhale A) \<omega> })"
-
-| RedExhaleFalse: "\<lbrakk> wd_assertion Pr RExhale A \<omega> ; \<not> Pr RExhale \<Turnstile> \<langle>A; \<omega>\<rangle> \<rbrakk> \<Longrightarrow> red_stmt conf Pr (Exhale A) \<omega> Failure"
-| RedAssertFailure: "\<lbrakk> \<not> wd_assertion Pr RExhale A \<omega> \<rbrakk> \<Longrightarrow> red_stmt conf Pr (Assert A) \<omega> Failure"
-| RedInhaleFailure: "\<lbrakk> \<not> wd_assertion Pr RInhale A \<omega> \<rbrakk> \<Longrightarrow> red_stmt conf Pr (Inhale A) \<omega> Failure"
-| RedExhaleFailure: "\<lbrakk> \<not> wd_assertion Pr RExhale A \<omega> \<rbrakk> \<Longrightarrow> red_stmt conf Pr (Exhale A) \<omega> Failure"
-*)
-
-(*
-(* | RedAssumeTrue: "\<lbrakk> wft Pr A \<omega> \<rbrakk> \<Longrightarrow> red_stmt conf Pr (Assume A) \<omega> (Set {\<omega>})"
-| RedAssumeFalse: "\<lbrakk> wd_assertion Pr RExhale A \<omega> ; \<not> Pr \<Turnstile> \<langle>A; \<omega>\<rangle> \<rbrakk> \<Longrightarrow> red_stmt conf Pr (Assume A) \<omega> (Set {})"
-| RedAssumeFailure: "\<lbrakk> \<not> wd_assertion Pr RExhale A \<omega> \<rbrakk> \<Longrightarrow> red_stmt conf Pr (Assume A) \<omega> Failure" *)
-
-| RedIfTrue: "\<lbrakk> Pr \<turnstile> \<langle>b ; \<omega>\<rangle> [\<Down>] Val (VBool True) ; red_stmt conf Pr s1 \<omega> r \<rbrakk> \<Longrightarrow> red_stmt conf Pr (If b s1 s2) \<omega> r"
-| RedIfFalse: "\<lbrakk> Pr \<turnstile> \<langle>b ; \<omega>\<rangle> [\<Down>] Val (VBool False) ; red_stmt conf Pr s2 \<omega> r \<rbrakk> \<Longrightarrow> red_stmt conf Pr (If b s1 s2) \<omega> r"
-| RedIfFailure: "\<lbrakk> Pr \<turnstile> \<langle>b ; \<omega>\<rangle> [\<Down>] VFailure \<rbrakk> \<Longrightarrow> red_stmt conf Pr (If b _ _) \<omega> Failure"
-
-(* May be an overapproximation, but should not be an issue, except maybe for the store *)
-| RedSeq: "\<lbrakk> red_stmt conf Pr s1 \<omega> (Set s) ; \<And>x. x \<in> s \<Longrightarrow> (\<exists>s'. red_stmt conf Pr s2 x (Set s') \<and> s' \<subseteq> r)  \<rbrakk> \<Longrightarrow> red_stmt conf Pr (Seq s1 s2) \<omega> (Set r)"
-| RedSeqFailure: "\<lbrakk> red_stmt conf Pr s1 \<omega> Failure \<rbrakk> \<Longrightarrow> red_stmt conf Pr (Seq s1 s2) \<omega> Failure"
-
-(* No need to handle the case where the variable is not defined, since it is part of well-definedness of a program *)
-| RedLocalAssign: "\<lbrakk> Pr \<turnstile> \<langle>e; (\<sigma>, \<gamma>)\<rangle> [\<Down>] (Val v) \<rbrakk> \<Longrightarrow> red_stmt conf Pr (LocalAssign x e) (\<sigma>, \<gamma>) (Set {(\<sigma>(x \<mapsto> v), \<gamma>)})"
-| RedLocalAssignFailure: "\<lbrakk> Pr \<turnstile> \<langle>e; \<omega>\<rangle> [\<Down>] VFailure \<rbrakk> \<Longrightarrow> red_stmt conf Pr (LocalAssign x e) \<omega> Failure"
-
-| RedFieldAssign: "\<lbrakk> Pr \<turnstile> \<langle>r; \<omega>\<rangle> [\<Down>] (Val (VRef (Address a))) ;  can_write (get_m \<omega>) (a, f) ; Pr \<turnstile> \<langle>e; \<omega>\<rangle> [\<Down>] (Val v) \<rbrakk>
-  \<Longrightarrow> red_stmt conf Pr (FieldAssign r f e) \<omega> (Set {field_assign \<omega> (a, f) v})"
-
-| RedFieldAssignFailureNull: "\<lbrakk> Pr \<turnstile> \<langle>r; \<omega>\<rangle> [\<Down>] (Val (VRef Null)) \<rbrakk> \<Longrightarrow> red_stmt conf Pr (FieldAssign r f e) \<omega> Failure"
-| RedFieldAssignFailurePerm: "\<lbrakk> Pr \<turnstile> \<langle>r; \<omega>\<rangle> [\<Down>] (Val (VRef (Address a))) ; \<not> (can_write (get_m \<omega>) (a, f)) \<rbrakk> \<Longrightarrow> red_stmt conf Pr (FieldAssign r f e) \<omega> Failure"
-| RedFieldAssignFailureRef: "\<lbrakk> Pr \<turnstile> \<langle>r; \<omega>\<rangle> [\<Down>] VFailure \<rbrakk> \<Longrightarrow> red_stmt conf Pr (FieldAssign r f e) \<omega> Failure"
-| RedFieldAssignFailureExp: "\<lbrakk> Pr \<turnstile> \<langle>e; \<omega>\<rangle> [\<Down>] VFailure \<rbrakk> \<Longrightarrow> red_stmt conf Pr (FieldAssign r f e) \<omega> Failure"
-
-
-(* Failure only when program not well-defined? *)
-| RedLabel: "red_stmt conf Pr (Label l) (\<sigma>, \<tau>, \<phi>) (Set {(\<sigma>, \<tau>(l \<mapsto> \<phi>), \<phi>)})"
-
-(* Overapproximation possible *)
-| RedScope: "\<lbrakk> \<And>\<sigma>'. \<sigma>' \<in> declare_var_list l \<sigma> \<Longrightarrow> (\<exists>s'. red_stmt conf Pr s (\<sigma>', \<tau>, \<phi>) (Set s') \<and> s' \<subseteq> r) \<rbrakk> \<Longrightarrow> red_stmt conf Pr (Scope l s) (\<sigma>, \<tau>, \<phi>) (Set (unshift_state (length l) ` r))"
-
-| RedFoldSkip: "\<lbrakk> equi_predicate conf ; \<not> ghost_assert conf\<rbrakk> \<Longrightarrow> red_stmt conf Pr (Fold _ _ _) \<omega> (Set {\<omega>})"
-| RedFoldAssert: "\<lbrakk> equi_predicate conf ; ghost_assert conf ;  red_stmt conf Pr (Assert (AccPredicate p l f)) \<omega> r \<rbrakk> \<Longrightarrow> red_stmt conf Pr (Fold p l f) \<omega> r"
-| RedUnfoldSkip: "\<lbrakk> equi_predicate conf ; \<not> ghost_assert conf\<rbrakk> \<Longrightarrow> red_stmt conf Pr (Unfold _ _ _) \<omega> (Set {\<omega>})"
-| RedUnfoldAssert: "\<lbrakk> equi_predicate conf ; ghost_assert conf ; red_stmt conf Pr (Assert (AccPredicate p l f)) \<omega> r \<rbrakk> \<Longrightarrow> red_stmt conf Pr (Unfold p l f) \<omega> r"
-
-| RedApplySkip: "\<lbrakk> equi_wands conf ; \<not> ghost_assert conf\<rbrakk> \<Longrightarrow> red_stmt conf Pr (Apply _ _) \<omega> (Set {\<omega>})"
-| RedApplyAssert: "\<lbrakk> equi_wands conf ; ghost_assert conf ; red_stmt conf Pr (Assert (A --* B)) \<omega> r\<rbrakk> \<Longrightarrow> red_stmt conf Pr (Apply A B) \<omega> (Set {\<omega>})"
-| RedPackageSkip: "\<lbrakk> equi_wands conf ; \<not> ghost_assert conf\<rbrakk> \<Longrightarrow> red_stmt conf Pr (Package _ _) \<omega> (Set {\<omega>})"
-| RedPackageAssert: "\<lbrakk> equi_wands conf ; ghost_assert conf ; red_stmt conf Pr (Assert (A --* B)) \<omega> r\<rbrakk> \<Longrightarrow> red_stmt conf Pr (Package A B) \<omega> (Set {\<omega>})"
-
-| RedWhileTrue: "\<lbrakk> Pr \<turnstile> \<langle>b ; \<omega>\<rangle> [\<Down>] Val (VBool True) ; red_stmt conf Pr s \<omega> (Set r1) ; \<And>x. x \<in> r1 \<Longrightarrow> (\<exists>r2'. red_stmt conf Pr (While b I s) x (Set r2') \<and> r2' \<subseteq> r2)\<rbrakk>
-  \<Longrightarrow> red_stmt conf Pr (While b I s) \<omega> (Set r2)"
-| RedWhileFalse: "\<lbrakk> Pr \<turnstile> \<langle>b ; \<omega>\<rangle> [\<Down>] Val (VBool False) \<rbrakk> \<Longrightarrow> red_stmt conf Pr (While b _ _) \<omega> (Set {\<omega>})"
-| RedWhileFailure: "\<lbrakk> Pr \<turnstile> \<langle>b ; \<omega>\<rangle> [\<Down>] VFailure \<rbrakk> \<Longrightarrow> red_stmt conf Pr (While b _ _) \<omega> Failure"
-
-(* Only rets and args defined when executing a method call, also empty trace *)
-(* If method does not exist, or wrong number of args or rets: Not well-defined *)
-(* Concrete method *)
-| RedMethod: "\<lbrakk> methods Pr name = Some m ; body m = Some s; length vals = length x ; list_all2 (\<lambda>xx v. \<sigma> xx = Some v) x vals ;
-  \<And>\<sigma>'. \<sigma>' \<in> declare_var_list (rets m) \<sigma> \<Longrightarrow> (\<exists>s'. red_stmt conf Pr s (shift_and_add_list \<sigma>' vals, \<phi>) (Set s') \<and> s' \<subseteq> r) \<rbrakk>
-  \<Longrightarrow> red_stmt conf Pr (MethodCall y name x) \<omega> (Set (unshift_state (length (args m)) ` r))"
-
-(* Abstract method *)
-definition ver :: "configuration \<Rightarrow> 'a program \<Rightarrow> stmt \<Rightarrow> 'a state \<Rightarrow> bool" where
-  "ver conf Pr s \<omega> \<longleftrightarrow> (\<exists>r. red_stmt conf Pr s \<omega> (Set r))"
+definition ver_total :: "'a program \<Rightarrow> conf \<Rightarrow> stmt \<Rightarrow> ('a full_total_state) set \<Rightarrow> bool" where
+  "ver Pr conf s \<omega> \<longleftrightarrow> (\<exists>r. red_stmt_total_single Pr conf s \<omega> (Set r))"
 *)
 
 end
